Modify parse table entry type

LL1/ParseTableGen.v
@@ -4,23 +4,25 @@ Require Import Lib.Grammar.
 
 Require Import LL1.ParseTable.
 
-Definition prod_la_pair := (production * lookahead)%type.
+Definition pt_entry := (nonterminal * lookahead * list symbol)%type.
 
-Lemma prod_la_pair_dec :
-  forall p p2 : prod_la_pair,
+Lemma pt_entry_dec :
+  forall p p2 : pt_entry,
     {p = p2} + {p <> p2}.
 Proof.
   repeat decide equality.
 Defined.
 
+(* Build a parse table from a (correct) list of parse table entries *)
+
 Definition empty_pt := ParseTable.empty (list symbol).
 
-Definition addEntry (p : prod_la_pair) (o : option parse_table) :=
+Definition addEntry (p : pt_entry) (o : option parse_table) :=
   match o with
   | None => None
   | Some tbl =>
     match p with
-    | ((x, gamma), la) =>
+    | (x, la, gamma) =>
       match pt_lookup x la tbl with
       | None => Some (pt_add x la gamma tbl)
       | Some gamma' =>
@@ -29,6 +31,6 @@ Definition addEntry (p : prod_la_pair) (o : option parse_table) :=
     end
   end.
 
-Definition mkParseTable (ps : list prod_la_pair) :=
+Definition mkParseTable (ps : list pt_entry) :=
   fold_right addEntry (Some empty_pt) ps.
 
